doc/book/code/Part5.Mapply.fst
@@ -15,12 +15,8 @@ assume val qr_s : unit -> Lemma (q ==> r ==> s)
 let test () : Lemma (requires p) (ensures s) =
   assert s by (
     mapply (`qr_s);
-    focus (fun () ->
-      mapply (`p_q);
-      smt());
-    focus (fun () ->
-      mapply (`p_r);
-      smt());
+    mapply (`p_q);
+    mapply (`p_r);
     ()
   )
 //SNIPPET_END: mapply
